Fixed completeness of the binop case for expressions

ImpE2.v
@@ -142,6 +142,19 @@ Section Semantics.
     (ecfg_exp2 ecfg, project_reg (ecfg_reg2 ecfg) is_left,
      project_mem (ecfg_mem2 ecfg) is_left).
 
+   Definition contains_nat (v : val2) :=
+     (exists n1, v = VSingle (Vnat n1)) \/
+     (exists n1 n2, v = VPair (Vnat n1) (Vnat n2)).
+
+   Fixpoint apply_op (op : nat -> nat -> nat) (v1 v2 : val2) :=
+     match v1, v2 with
+     | VSingle (Vnat n1), VSingle (Vnat n2) => VSingle (Vnat (op n1 n2))
+     | VSingle (Vnat n1), VPair (Vnat n2) (Vnat n3) => VPair (Vnat (op n1 n2)) (Vnat (op n1 n3))
+     | VPair (Vnat n1) (Vnat n2), VPair (Vnat n3) (Vnat n4) =>
+                                  VPair (Vnat (op n1 n3)) (Vnat (op n2 n4))
+     | _, _ => v1
+     end.
+   
   Inductive estep2 : esemantics2 :=
   | Estep2_nat : forall md d ecfg n,
       ecfg_exp2 ecfg = Enat n ->
@@ -156,11 +169,12 @@ Section Semantics.
       ecfg_exp2 ecfg = Evar x ->
       ecfg_reg2 ecfg x = v ->
       estep2 md d ecfg v
-  | Estep2_binop : forall md d ecfg e1 e2 n1 n2 op,
+  | Estep2_binop : forall md d ecfg e1 e2 v1 v2 op,
       ecfg_exp2 ecfg = Ebinop e1 e2 op ->
-      estep2 md d (ecfg_update_exp2 ecfg e1) (VSingle (Vnat n1)) ->
-      estep2 md d (ecfg_update_exp2 ecfg e2) (VSingle (Vnat n2)) ->
-      estep2 md d ecfg (VSingle (Vnat (op n1 n2)))
+      estep2 md d (ecfg_update_exp2 ecfg e1) v1 ->
+      estep2 md d (ecfg_update_exp2 ecfg e2) v2 ->
+      contains_nat v1 /\ contains_nat v2 ->
+      estep2 md d ecfg (apply_op op v1 v2)
   | Estep2_deref : forall md d ecfg e r m l v,
       ecfg = (Ederef e, r, m) ->
       estep2 md d (e, r, m) (VSingle (Vloc l)) ->
